new_counter_spec2

theories/coneris/examples/random_counter/impl2.v
@@ -97,15 +97,15 @@ Section impl2.
   Class counterG2 Σ := CounterG2 { counterG2_error::hocap_errorGS Σ;
                                    counterG2_tapes:: hocap_tapesGS' Σ;
                                    counterG2_frac_authR:: inG Σ (frac_authR natR);
-                                   counterG2_flipG:: flipG Σ
+                                   counterG2_flipG: flipG Σ
                          }.
   
-  Context `{!conerisGS Σ, !hocap_errorGS Σ, !hocap_tapesGS' Σ, !inG Σ (frac_authR natR), L:flipG Σ}.
+  Context `{L:!flipG Σ, !hocap_errorGS Σ, !hocap_tapesGS' Σ, !inG Σ (frac_authR natR)}.
   
   
-  Definition counter_inv_pred2 (c:val) γ1 γ2 γ3:=
-    (∃ (ε:R) (m:gmap loc (bool*list nat)) (l:loc) (z:nat) γ1' γ2' N',
-        is_flip (L:=L) N' γ1' γ2' ∗
+  Definition counter_inv_pred2 N (c:val) γ1 γ2 γ3:=
+    (∃ (ε:R) (m:gmap loc (bool*list nat)) (l:loc) (z:nat) γ1' γ2',
+        is_flip (L:=L) (N.@"flip") γ1' γ2' ∗
         flip_error_frag (L:=L) γ1' ε ∗ ●↯ ε @ γ1 ∗
         ([∗ map] α ↦ t ∈ m, flip_tapes_frag (L:=L) γ2' α (if t.1:bool then nat_to_bool <$> (expander t.2) else nat_to_bool <$> (drop 1%nat (expander t.2))) ) 
         ∗ ●m@γ2 ∗  
@@ -116,28 +116,30 @@ Section impl2.
     {{{ ↯ ε }}}
       new_counter2 #() @ E
       {{{ (c:val), RET c;
-          ∃ γ1 γ2 γ3, inv N (counter_inv_pred2 c γ1 γ2 γ3) ∗
+          ∃ γ1 γ2 γ3, inv (N.@ "counter") (counter_inv_pred2 N c γ1 γ2 γ3) ∗
                       ◯↯ε @ γ1 ∗ own γ3 (◯F 0%nat)
       }}}.
   Proof.
-  Admitted.
-  (*   rewrite /new_counter2. *)
-  (*   iIntros (Φ) "Hε HΦ". *)
-  (*   wp_pures. *)
-  (*   wp_alloc l as "Hl". *)
-  (*   iDestruct (ec_valid with "[$]") as "%". *)
-  (*   unshelve iMod (hocap_error_alloc (mknonnegreal ε _)) as "[%γ1 [H1 H2]]". *)
-  (*   { lra. } *)
-  (*   simpl. *)
-  (*   iMod (hocap_tapes_alloc' (∅:gmap _ _)) as "[%γ2 [H3 H4]]". *)
-  (*   iMod (own_alloc (●F 0%nat ⋅ ◯F 0%nat)) as "[%γ3[H5 H6]]". *)
-  (*   { by apply frac_auth_valid. } *)
-  (*   replace (#0) with (#0%nat) by done. *)
-  (*   iMod (inv_alloc N _ (counter_inv_pred2 (#l) γ1 γ2 γ3) with "[$Hε $Hl $H1 $H3 $H5]") as "#Hinv". *)
-  (*   { iSplit; last done. by iApply big_sepM_empty. } *)
-  (*   iApply "HΦ". *)
-  (*   iExists _, _, _. by iFrame. *)
-  (* Qed. *)
+    rewrite /new_counter2.
+    iIntros (Φ) "Hε HΦ".
+    wp_pures.
+    iDestruct (ec_valid with "[$]") as "%".
+    iMod (flip_inv_create_spec with "[$]") as "(%γ1'&%γ2'&#?&Hε)".
+    wp_alloc l as "Hl".
+    unshelve iMod (hocap_error_alloc (mknonnegreal ε _)) as "[%γ1 [H1 H2]]".
+    { lra. }
+    simpl.
+    iMod (hocap_tapes_alloc' (∅:gmap _ _)) as "[%γ2 [H3 H4]]".
+    iMod (own_alloc (●F 0%nat ⋅ ◯F 0%nat)) as "[%γ3[H5 H6]]".
+    { by apply frac_auth_valid. }
+    replace (#0) with (#0%nat) by done.
+    iMod (inv_alloc (N.@"counter") _ (counter_inv_pred2 N (#l) γ1 γ2 γ3) with "[$Hε $Hl $H1 $H3 $H5]") as "#Hinv".
+    { iNext. iExists _. iSplit; first done.
+      iSplit; last done.
+      by iApply big_sepM_empty. }
+    iApply "HΦ".
+    iExists _, _, _. by iFrame.
+  Qed.
 
 
   (** This lemma is not possible as only one view shift*)
@@ -164,7 +166,7 @@ Section impl2.
 
   Lemma allocate_tape_spec2 N E c γ1 γ2 γ3:
     ↑N ⊆ E->
-    {{{ inv N (counter_inv_pred2 c γ1 γ2 γ3) }}}
+    {{{ inv (N.@ "counter") (counter_inv_pred2 N c γ1 γ2 γ3) }}}
       allocate_tape2 #() @ E
       {{{ (v:val), RET v;
           ∃ (α:loc), ⌜v=#lbl:α⌝ ∗ α ◯↪N (true,  []) @ γ2
@@ -189,7 +191,7 @@ Section impl2.
 
   Lemma incr_counter_tape_spec_some2 N E c γ1 γ2 γ3 (P: iProp Σ) (Q:nat->iProp Σ) (α:loc) (n:nat) ns:
     ↑N⊆E ->
-    {{{ inv N (counter_inv_pred2 c γ1 γ2 γ3) ∗
+    {{{ inv (N.@ "counter") (counter_inv_pred2 N c γ1 γ2 γ3) ∗
         □ (∀ (z:nat), P ∗ own γ3 (●F z) ={E∖↑N}=∗
                           own γ3 (●F(z+n)%nat)∗ Q z) ∗
         P ∗ α ◯↪N (true, n::ns) @ γ2
@@ -255,14 +257,14 @@ Section impl2.
   (*   by iFrame. *)
   (* Qed. *)
 
-  Lemma counter_presample_spec2 NS  E ns α
+  Lemma counter_presample_spec2 N  E ns α
      (ε2 : R -> nat -> R)
     (P : iProp Σ) T γ1 γ2 γ3 c:
-    ↑NS ⊆ E ->
+    ↑N ⊆ E ->
     (∀ ε n, 0<= ε -> 0<=ε2 ε n)%R ->
     (∀ (ε:R), 0<= ε ->SeriesC (λ n, if (bool_decide (n≤3%nat)) then 1 / (S 3%nat) * ε2 ε n else 0%R)%R <= ε)%R->
-    inv NS (counter_inv_pred2 c γ1 γ2 γ3) -∗
-    (□∀ (ε:R) n, (P ∗ ●↯ ε@ γ1) ={E∖↑NS}=∗
+    inv (N.@ "counter") (counter_inv_pred2 N c γ1 γ2 γ3) -∗
+    (□∀ (ε:R) n, (P ∗ ●↯ ε@ γ1) ={E∖↑N}=∗
         (⌜(1<=ε2 ε n)%R⌝ ∨(●↯ (ε2 ε n) @ γ1 ∗ T (n))))
         -∗
     P -∗ α ◯↪N (true, ns) @ γ2 -∗
@@ -355,7 +357,7 @@ Section impl2.
 
   Lemma read_counter_spec2 N E c γ1 γ2 γ3 P Q:
     ↑N ⊆ E ->
-    {{{  inv N (counter_inv_pred2 c γ1 γ2 γ3) ∗
+    {{{  inv (N.@ "counter") (counter_inv_pred2 N c γ1 γ2 γ3) ∗
         □ (∀ (z:nat), P ∗ own γ3 (●F z) ={E∖↑N}=∗
                     own γ3 (●F z)∗ Q z)
          ∗ P
@@ -386,7 +388,7 @@ Program Definition random_counter2 `{!conerisGS Σ, flip_spec Σ}: random_counte
     error_name := gname;
     tape_name := gname;
     counter_name :=gname;
-    is_counter _ N c γ1 γ2 γ3 := inv N (counter_inv_pred2 (L:=_) c γ1 γ2 γ3);
+    is_counter _ N c γ1 γ2 γ3 := inv (N.@ "counter") (counter_inv_pred2 (L:=_) N c γ1 γ2 γ3);
     counter_error_auth _ γ x := ●↯ x @ γ;
     counter_error_frag _ γ x := ◯↯ x @ γ;
     counter_tapes_auth _ γ m := (●((λ ns, (true, ns))<$>m)@γ)%I;
@@ -480,3 +482,4 @@ Next Obligation.
   apply nat_local_update. lia.
 Qed.
   
+
